new version of correctness proof, a little bit more complete

src/ExpandWhens_r.v
@@ -795,6 +795,23 @@ There may be numbers that are projected to 0. *)
    (* combines component declarations in the two branches. *)
       OK (CE.map2 combine_branches_ce_map2_helper ce_true ce_false).
 
+Definition ce_map_difference_helper (minuend_entry subtrahend_entry : option (cmpnt_init_typs * fcomponent)) : option (cmpnt_init_typs * fcomponent) :=
+match subtrahend_entry with
+| Some _ => None
+| None => minuend_entry
+end.
+
+Definition ce_map_intersection_helper (entry1 entry2 : option (cmpnt_init_typs * fcomponent)) : option (cmpnt_init_typs * fcomponent) :=
+match entry1, entry2 with
+| Some _, Some _ => entry1
+| _, _ => None
+end.
+
+Definition ce_has_no_double_declarations (ce_butlast ce_true ce_false : CE.env) : bool :=
+   (* checks whether there are double declarations in the component environments *)
+   CE.is_empty (CE.map2 ce_map_intersection_helper (CE.map2 ce_map_difference_helper ce_true ce_butlast)
+                                                   (CE.map2 ce_map_difference_helper ce_false ce_butlast)).
+
    Fixpoint expandBranch_precondition_declarations (ss : hfstmt_seq) (ce_other_modules : CE.env) (ce_previous : CE.env) : @error_type CE.env :=
    (* If all declarations are ground types, there are no partial connects in ss,
       and all full connects concern ground types,
@@ -855,7 +872,9 @@ There may be numbers that are projected to 0. *)
                      expandBranch_precondition_declarations ss_false ce_other_modules ce_butlast_result with
                | Err e, _ | _, Err e => Err e
                | OK ce_true_result, OK ce_false_result =>
-                    combine_branches_ce ce_true_result ce_false_result
+                    if ce_has_no_double_declarations ce_butlast_result ce_true_result ce_false_result
+                    then combine_branches_ce ce_true_result ce_false_result
+                    else Err Ealready_declared
                end
           | _ => OK ce_butlast_result
                  (* for Sinst, one has to check ce_other_modules as well.
@@ -1067,6 +1086,7 @@ Proof.
       destruct (expandBranch_precondition_declarations ss_false ce_other_modules e) as [e_false|] ;
             try done.
       specialize IHss_true with (ce_declarations := e_true).
+      destruct (ce_has_no_double_declarations e e_true e_false) ; try done.
       unfold combine_branches_ce in H0.
       injection H0 ; clear H0 ; intro.
       rewrite -H CE.map2_1.
@@ -1095,8 +1115,10 @@ Qed.
    => forall id : VarOrder.T,
       if ref2var (Eid id) is OK var
       then match CE.find var ce_declarations with
-           | Some (Aggr_typ t, _) => expandBranch_one_component_sem_conform (Eid id) t ss cm_result cm_previous
-           | Some (Reg_typ reg, _) => expandBranch_one_component_sem_conform (Eid id) (type reg) ss cm_result cm_previous
+           | Some (Aggr_typ t, fcomp) => if orient_of_comp fcomp == Source
+                                         then expandBranch_one_component_sem_conform_flipped (Eid id) t ss cm_result cm_previous
+                                         else expandBranch_one_component_sem_conform (Eid id) t ss cm_result cm_previous
+           | Some (Reg_typ reg,_) => expandBranch_one_component_sem_conform (Eid id) (type reg) ss cm_result cm_previous
            | Some (Mem_typ mem, _) => if type_of_mem mem is OK tom
                                       then expandBranch_one_component_sem_conform_flipped (Eid id) tom ss cm_result cm_previous
                                       else false
@@ -1333,6 +1355,10 @@ Proof.
       specialize IHss' with (var := var) ;
       specialize IHss_true' with (var := var) ;
       specialize IHss_false' with (var := var).
+      destruct (ce_has_no_double_declarations ce_before ce_true ce_false) eqn: Hno_double_declarations ; try done.
+      unfold combine_branches_ce in H0.
+      unfold combine_branches in H1.
+      injection H0 ; injection H1 ; clear H0 H1 ; intros H1 _ H0.
       destruct (CE.find var ce_before) as [p_before|] eqn: Hfind_before.
       * (* the component was declared before the Swhen statement. *)
         (* We can use expandBranch_precondition_declarations_does_not_redefine
@@ -1348,9 +1374,6 @@ Proof.
         rewrite H2 in IHss_true'.
         rewrite H3 in IHss_false'.
         destruct p_before as [comp_typ_before fcomp_before].
-        unfold combine_branches_ce in H0.
-        unfold combine_branches in H1.
-        injection H0 ; injection H1 ; clear H0 H1 ; intros H1 _ H0.
         rewrite -H0 CE.map2_1 ;
               try (left ;
                    unfold CE.In ;
@@ -1405,9 +1428,6 @@ Proof.
             apply CE.find_2, Hfind_true.
       destruct (CE.find var ce_true) eqn: Hfind_true.
       * (* the component was declared in the true branch. *)
-        unfold combine_branches_ce in H0.
-        unfold combine_branches in H1.
-        injection H0 ; injection H1 ; clear H0 H1 ; intros H1 _ H0.
         rewrite -H0 CE.map2_1 ;
               try (left ;
                    unfold CE.In ;
@@ -1415,9 +1435,33 @@ Proof.
                    apply CE.find_2, Hfind_true).
         rewrite /combine_branches_ce_map2_helper Hfind_true -H1.
         destruct p as [comp_typ_true fcomp_true].
-        assert (CE.find var ce_false = None) by admit.
+        assert (CE.find var ce_false = None).
               (* should follow from type correctness of declarations:
                  a component cannot be declared in both branches of a Swhen statement *)
+              apply CE.is_empty_2 in Hno_double_declarations.
+              unfold CE.Empty in Hno_double_declarations.
+              destruct (CE.find var ce_false) eqn: Hfind_false ; try done.
+              destruct p as [comp_typ_false fcomp_false].
+              specialize Hno_double_declarations with (a := var) (e := (comp_typ_true, fcomp_true)).
+              contradict Hno_double_declarations.
+              apply CE.find_2.
+              rewrite CE.map2_1.
+              + rewrite CE.map2_1 ;
+                      try (left ; exists (comp_typ_true, fcomp_true) ;
+                           apply CE.find_2, Hfind_true).
+                rewrite CE.map2_1 ;
+                      try (left ; exists (comp_typ_false, fcomp_false) ;
+                           apply CE.find_2, Hfind_false).
+                rewrite Hfind_true Hfind_false Hfind_before
+                        /ce_map_difference_helper
+                        /ce_map_intersection_helper //.
+              + left.
+                exists (comp_typ_true, fcomp_true).
+                apply CE.find_2.
+                rewrite CE.map2_1 ;
+                      try (left ; exists (comp_typ_true, fcomp_true) ;
+                           apply CE.find_2, Hfind_true).
+                rewrite /ce_map_difference_helper Hfind_before Hfind_true //.
         rewrite H2 in IHss_false'.
         destruct (orient_of_comp fcomp_true == Source).
         + (* the component has source orientation, so it should not appear anywhere.
@@ -1462,9 +1506,6 @@ Proof.
             apply CE.find_2, Hfind_cm_true.
       destruct (CE.find var ce_false) eqn: Hfind_false.
       * (* the component was declared in the false branch. *)
-        unfold combine_branches_ce in H0.
-        unfold combine_branches in H1.
-        injection H0 ; injection H1 ; clear H0 H1 ; intros H1 _ H0.
         rewrite -H0 CE.map2_1 ;
               try (right ;
                    unfold CE.In ;
@@ -1500,7 +1541,6 @@ Proof.
              so it is also afterwards. *)
           split ; try done.
           assert (CE.find var cm_result_false <> None).
-                (* Probably there exists a more elegant proof than the following... *)
                 move /eqP => H4.
                 apply IHss_false' in H4 ; done.
           rewrite CE.map2_1.
@@ -1513,9 +1553,6 @@ Proof.
             exists d.
             apply CE.find_2, Hfind_cm_false.
       * (* the component was not declared anywhere. *)
-        unfold combine_branches_ce in H0.
-        unfold combine_branches in H1.
-        injection H0 ; injection H1 ; clear H0 H1 ; intros H1 _ H0.
         rewrite -H0 -H1.
         destruct (CE.find var (CE.map2 combine_branches_ce_map2_helper ce_true ce_false)) eqn: Hfind_after.
         + assert (CE.In var ce_true \/ CE.In var ce_false)
@@ -1555,413 +1592,583 @@ Admitted.
    If ...
    then expandBranch_sem_conform is true. *)
 
-Definition expandBranch_correct_hfstmt_seq (ss : hfstmt_seq) : Prop :=
-   forall (ce_other_modules ce_previous_declarations : CE.env),
-      expandBranch_sem_conform ss ce_other_modules ce_previous_declarations empty_cmap.
-
-Definition expandBranch_correct_hfstmt (s : hfstmt) : Prop :=
-   if s is Swhen _ sst ssf
-   then expandBranch_correct_hfstmt_seq sst /\ expandBranch_correct_hfstmt_seq ssf
-   else True.
+Definition expandBranch_correct_hfstmt_seq (ce_other_modules : CE.env) (ss : hfstmt_seq) : Prop :=
+   forall (ce_previous_declarations : CE.env) (cm_previous : cmap),
+      expandBranch_fun_declarations_correspondence ce_previous_declarations cm_previous ->
+         expandBranch_sem_conform ss ce_other_modules ce_previous_declarations cm_previous.
 
 Theorem expandBranch_correct :
-   forall (ss : hfstmt_seq), expandBranch_correct_hfstmt_seq ss.
+   forall (ce_other_modules : CE.env) (ss : hfstmt_seq), expandBranch_correct_hfstmt_seq ce_other_modules ss
 (* Programs that cannot be handled by expandBranch_fun and generate an error message
    are always regarded as correct.
    Perhaps this will need to be refined later. *)
+with expandBranch_correct_Swhen :
+   forall (ce_other_modules : CE.env) (s : hfstmt),
+      if s is Swhen _ ss_true ss_false
+      then    expandBranch_correct_hfstmt_seq ce_other_modules ss_true
+           /\ expandBranch_correct_hfstmt_seq ce_other_modules ss_false
+      else True.
 Proof.
-apply hfstmt_seq_hfstmt_ind with (P := expandBranch_correct_hfstmt_seq)
-                                 (P0 := expandBranch_correct_hfstmt)
-      ; try done.
-all: unfold expandBranch_correct_hfstmt_seq, expandBranch_correct_hfstmt.
-all: unfold expandBranch_sem_conform.
-all: intros.
-* unfold expandBranch_precondition_declarations, expandBranch_fun, ref2var.
-  intro.
-  destruct (CE.find (nat_to_var (id * 3 + 1)) ce_previous_declarations) eqn: Hfind ; try done.
-  destruct p as [comp_typ f].
-  destruct comp_typ as [ft|reg|mem|]; try done.
-  + assert (exists t : fgtyp, ft = Gtyp t) by admit.
-    destruct H0 as [t].
-    rewrite H0.
-    simpl expandBranch_one_component_sem_conform.
-    (* the empty map does not contain any elements *)
-    done.
-  + (* register is similar to variable *)
-    admit.
-  + (* memory is similar to variable *)
-    admit.
-* specialize H with (ce_other_modules := ce_other_modules)
-                    (ce_previous_declarations := ce_previous_declarations).
-  assert (match expandBranch_precondition_declarations h ce_other_modules ce_previous_declarations with
-          | OK ce_declarations =>
-               match expandBranch_fun h ce_other_modules empty_cmap with
-               | OK (_, cm_result) => forall id : VarOrder.T,
-                    match ref2var (Eid id) with
-                    | OK var =>
-                         match CE.find var ce_declarations with
-                         | Some (@Aggr_typ _ t, _) =>
-                              expandBranch_one_component_sem_conform (Eid id) t h cm_result empty_cmap
-                         | Some (Reg_typ reg, _) =>
-                              expandBranch_one_component_sem_conform (Eid id) (type reg) h cm_result empty_cmap
-                         | Some (Mem_typ mem, _) =>
-                              match type_of_mem mem with
-                              | OK tom =>
-                                   expandBranch_one_component_sem_conform_flipped (Eid id) tom h cm_result empty_cmap
-                              | Err _ => false
-                              end
-                         | _ => true
-                         end
-                    | Err _ => true
-                    end
-               | Err _ => true
-               end
-          | Err _ => true
-          end) by (apply H, H1).
-  clear H.
-  simpl expandBranch_precondition_declarations.
-  destruct (expandBranch_precondition_declarations h ce_other_modules ce_previous_declarations) as [ce_declarations|] eqn: Hdeclarations ; try done.
-  destruct h0 eqn: Hstmt ; try done.
-  + (* Skip *)
-    simpl expandBranch_fun.
-    destruct (expandBranch_fun h ce_other_modules empty_cmap) ; try done.
-    destruct p as [_ cm_result].
+* clear expandBranch_correct.
+  induction ss ;
+  unfold expandBranch_correct_hfstmt_seq, expandBranch_sem_conform ;
+  intros.
+  + unfold expandBranch_precondition_declarations, expandBranch_fun, ref2var.
     intro.
-    specialize H2 with (id := id).
-    unfold ref2var ; unfold ref2var in H2.
-    destruct (CE.find (nat_to_var (id * 3 + 1)) ce_declarations) eqn: Hfind ; try done.
-    destruct p as [comp_typ fcomp].
-    destruct comp_typ as [ft|reg|mem|] ; try done.
+    destruct (CE.find (nat_to_var (id * 3 + 1)) ce_previous_declarations) eqn: Hfind ; try done.
+    destruct p as [comp_typ f].
+    destruct comp_typ as [ft|reg|mem|]; try done.
     - assert (exists t : fgtyp, ft = Gtyp t) by admit.
-      destruct H.
-      rewrite H ; rewrite H in H2.
-      unfold expandBranch_one_component_sem_conform, ref2var ;
-      unfold expandBranch_one_component_sem_conform, ref2var in H2.
-      simpl expandBranch_one_var_sem.
-      replace (CE.find (nat_to_var (id * 3 + 1)) empty_cmap) with (@None def_expr) in H2 by (done).
-      exact H2.
+      destruct H1 as [t].
+      rewrite H1.
+      destruct (orient_of_comp f == Source) ; try done.
+      simpl expandBranch_one_component_sem_conform.
+      destruct (CE.find (nat_to_var (id * 3 + 1)) cm_previous) ; try done.
+      destruct d ; done.
     - (* register is similar to variable *)
       admit.
     - (* memory is similar to variable *)
       admit.
-  + (* Swire *)
-    assert (exists t : fgtyp, f = Gtyp t) by admit.
-    destruct H.
-    rewrite H.
-    destruct (CE.find (nat_to_var (s * 3 + 1)) ce_declarations) eqn: Halready_declared ; try done.
-    simpl expandBranch_fun.
-    destruct (expandBranch_fun h ce_other_modules empty_cmap) ; try done.
-    destruct p as [_ cm_result].
-    intro.
-    specialize H2 with (id := id).
-    unfold ref2var ; unfold ref2var in H2.
-    destruct (eqVneq s id).
-    - rewrite e.
-      rewrite CELemmas.find_add_eq ; try rewrite /CE.SE.eq eq_refl //.
-      unfold aggr_typ, expandBranch_one_component_sem_conform, ref2var.
-      rewrite CELemmas.find_add_eq ; try rewrite /CE.SE.eq eq_refl //.
-      simpl expandBranch_one_var_sem.
-      rewrite eq_refl /expr_tree_to_def_expr eq_refl //.
-    - assert (forall val (ce : CE.env), CE.find (nat_to_var (id * 3 + 1))
-                      (CE.add (nat_to_var (s * 3 + 1)) val ce)
-             = CE.find (nat_to_var (id * 3 + 1)) ce).
-            intros.
-            apply CELemmas.find_add_neq.
-            clear -i.
-            unfold CE.SE.eq, nat_to_var.
-            move /eqP : i => i.
-            contradict i.
-            move /eqP : i => i.
-            assert (injective bin_of_nat)
-                  by (apply can_inj with (g := nat_of_bin),
-                            bin_of_natK).
-            unfold injective in H.
-            apply H in i.
-            move /eqP : i => i.
-            rewrite eqn_add2r eqn_mul2r orFb in i.
-            move /eqP : i => i.
-            assert (injective nat_of_bin)
-                  by (apply can_inj with (g := bin_of_nat),
-                            nat_of_binK).
-            unfold injective in H0.
-            apply H0 in i.
-            done.
-      rewrite H3.
-      destruct (CE.find (nat_to_var (id * 3 + 1)) ce_declarations) ; try done.
-      destruct p as [comp_typ fcomp].
-      destruct comp_typ as [ft|reg|mem|] ; try done.
-      * assert (exists t : fgtyp, ft = Gtyp t) by admit.
-        destruct H4.
-        rewrite H4 ; rewrite H4 in H2.
-        unfold expandBranch_one_component_sem_conform, ref2var ;
-        unfold expandBranch_one_component_sem_conform, ref2var in H2.
-        simpl expandBranch_one_var_sem.
-        replace (CE.find (nat_to_var (id * 3 + 1)) empty_cmap) with (@None def_expr) in H2 by (done).
-        replace (CE.find (nat_to_var (id * 3 + 1))
-        (CE.add (nat_to_var (s * 3 + 1))
-           D_undefined cm_result))
-        with (CE.find (nat_to_var (id * 3 + 1)) cm_result)
-        by admit. (* same proof as above, assertion H2 *)
-        apply negbTE in i.
-        rewrite (eq_sym id) i.
-        exact H2.
-      * (* register is similar to variable *)
-        admit.
-      * (* memory is similar to variable *)
-        admit.
-  + (* Sreg *)
-    (* Sreg is similar to Swire *)
-    admit.
-  + (* Smem *)
-    (* Smem is similar to Swire *)
-    admit.
-  + (* Sinst s s0, i.e. s = identifier and s0 = type of the module. *)
-    simpl expandBranch_fun.
-    destruct (expandBranch_fun h ce_other_modules empty_cmap) eqn: Hebf ;
-          try (destruct (CE.find s0 ce_other_modules) ;
-               try done ;
-               destruct p, c, f, (CE.find (nat_to_var (s * 3 + 1)) ce_declarations) ;
-               done).
-    destruct p as [ss_result cm_result].
-    destruct (CE.find s0 ce_other_modules) eqn: Hs0 ; try done.
-    destruct p as [ss_result0 cm_result0].
-    destruct ss_result0 ; try done.
-    destruct cm_result0 ; try done.
-    destruct (CE.find (nat_to_var (s * 3 + 1)) ce_declarations) eqn: Hs ; try done.
-    destruct (init_instance s s0 ce_other_modules cm_result) eqn: Hinit_instance ; try done.
-    intro.
-    specialize H2 with (id := id).
-    unfold ref2var ; unfold ref2var in H2.
-    destruct (eqVneq s id).
-    - (* id now does not have a ground type but is part of the instance.
-         That means, it has type (Btyp ...) where each field has a ground type. *)
-      rewrite !e CELemmas.find_add_eq ; try rewrite /CE.SE.eq eq_refl //.
-      rewrite e in Hinit_instance.
-      unfold aggr_typ.
-      (* Now we should argue as follows:
-         1. (to simplify) the type f is some (Btyp f0),
-            where f0 is a list of ground type entries.
-            (This should be based on H1 and Hs0.)
-         2. induction over f0. *)
-      unfold expandBranch_precondition_ce in H1.
-      specialize H1 with (id := s0).
-      unfold init_instance in Hinit_instance.
-      destruct (CE.find s0 ce_other_modules) ; try done.
-      destruct p.
-      destruct c0, f0 ; try discriminate.
-      destruct f1 ; try done.
-      injection Hs0 ; intro Hf0 ; clear Hs0.
-      rewrite -Hf0 ; clear Hf0 f.
-      simpl expandBranch_one_component_sem_conform.
-      move : H1 c Hinit_instance.
-      simpl init_ref.
-      induction f0.
-      * intros.
-        unfold expandBranch_one_component_sem_conform_fields ; done.
-      * simpl expandBranch_precondition_ce_module_fields ; intros.
-        destruct f0 ; try done.
-        simpl expandBranch_one_component_sem_conform_fields.
-        simpl init_ref_bundle in Hinit_instance.
-        destruct f.
-        + apply IHf0 ; try done.
-          destruct (init_ref_bundle (Eid id) f1 Sink cm_result) ; done.
-        + rewrite eq_refl /expr_tree_to_def_expr /var_to_nat bin_of_natK.
-          rewrite /var_to_nat bin_of_natK in Hinit_instance.
-          destruct (init_ref_bundle (Eid id) f1 Sink
-                     cm_result) eqn: Hirb ; try done.
-          injection Hinit_instance ; clear Hinit_instance ; intro Hinit_instance.
-          rewrite -{1}Hinit_instance CELemmas.find_add_eq ;
-                try rewrite /CE.SE.eq eq_refl //.
-          rewrite andTb.
-          specialize IHf0 with (c := c0).
-          (* Now, because f1 does not contain field v,
-             we can use IHf0 to prove the semantic conformity. *)
-          admit.
-    - rewrite CELemmas.find_add_neq.
-      * (* This can be proven using H2 and Hinit_instance.
-           Similar to the above, we use that s != id and therefore
-           the relevant parts of cm_result and c are equal. *)
-        admit.
-      * rewrite /CE.SE.eq /nat_to_var.
-        move /eqP : i => i ; contradict i ; move /eqP : i => i.
-        assert (id * 3 + 1 == s * 3 + 1) by (rewrite -(bin_of_natK (id * 3 + 1)) i bin_of_natK eq_refl //).
-        rewrite addn1 addn1 eqSS eqn_pmul2r // in H.
-        move /eqP : H => H.
-        rewrite -(nat_of_binK id) H nat_of_binK ; reflexivity.
-  + (* Snode s h1 *)
-    simpl expandBranch_fun.
-    destruct (expandBranch_fun h ce_other_modules empty_cmap) ; try done.
-    destruct p as [ss_result cm_result].
-    (* expandBranch_one_component_sem_conform ignores the Snode statement,
-       so it should be possible to prove this based on H2. *)
-    admit.
-  + (* Sfcnct h1 h2 *)
-    simpl expandBranch_fun.
-    destruct (ref2var h1) eqn: Hh1 ; try done.
-    destruct (CE.find s ce_declarations) eqn: Hfinds ; try done.
-    destruct p as [comp_typ_s fcomp_s].
-    destruct comp_typ_s ; try done.
-    destruct f ; try done.
-    destruct (expandBranch_fun h ce_other_modules empty_cmap) ; try done.
-    destruct p as [ss_result cm_result].
-    intro.
-    specialize H2 with (id := id).
-    destruct (eqVneq (Eid id) h1).
-    - rewrite e Hh1 ; rewrite e Hh1 in H2.
-      destruct (CE.find s ce_declarations) ; try done.
-      destruct p as [comp_typ fcomp].
-      injection Hfinds ; clear Hfinds ; intros.
-      rewrite H3 ; rewrite H3 in H2.
-      simpl expandBranch_one_component_sem_conform.
-      rewrite Hh1 CELemmas.find_add_eq ; try (unfold CE.SE.eq ; done).
-      rewrite eq_refl /expr_tree_to_def_expr eq_refl //.
-    - unfold ref2var ; unfold ref2var in H2.
+  + unfold expandBranch_correct_hfstmt_seq in IHss.
+    assert (IHss' : match expandBranch_precondition_declarations ss ce_other_modules ce_previous_declarations with
+                    | OK ce_declarations =>
+                        match expandBranch_fun ss ce_other_modules cm_previous with
+                        | OK (_, cm_result) =>
+                            forall id : VarOrder.T,
+                            match ref2var (Eid id) with
+                            | OK var =>
+                                match CE.find var ce_declarations with
+                                | Some (@Aggr_typ _ t, fcomp) =>
+                                    if orient_of_comp fcomp == Source
+                                    then expandBranch_one_component_sem_conform_flipped (Eid id) t ss cm_result cm_previous
+                                    else expandBranch_one_component_sem_conform (Eid id) t ss cm_result cm_previous
+                                | Some (Reg_typ reg, _) =>
+                                    expandBranch_one_component_sem_conform (Eid id) (type reg) ss cm_result cm_previous
+                                | Some (Mem_typ mem, _) =>
+                                    match type_of_mem mem with
+                                    | OK tom =>
+                                        expandBranch_one_component_sem_conform_flipped (Eid id) tom ss cm_result cm_previous
+                                    | Err _ => false
+                                    end
+                                | _ => true
+                                end
+                            | Err _ => true
+                            end
+                        | Err _ => true
+                        end
+                    | Err _ => true
+                    end)
+          by (apply IHss ; done).
+    clear IHss.
+    simpl expandBranch_precondition_declarations.
+    destruct (expandBranch_precondition_declarations ss ce_other_modules ce_previous_declarations) as [ce_declarations|] eqn: Hdeclarations ; try done.
+    destruct h eqn: Hstmt ; try done.
+    - (* Skip *)
+      simpl expandBranch_fun.
+      destruct (expandBranch_fun ss ce_other_modules cm_previous) ; try done.
+      destruct p as [_ cm_result].
+      intro.
+      specialize IHss' with (id := id).
+      unfold ref2var ; unfold ref2var in IHss'.
       destruct (CE.find (nat_to_var (id * 3 + 1)) ce_declarations) eqn: Hfind ; try done.
       destruct p as [comp_typ fcomp].
       destruct comp_typ as [ft|reg|mem|] ; try done.
-      * assert (exists t : fgtyp, ft = Gtyp t) by admit.
-        destruct H as [t].
-        rewrite H ; rewrite H in H2.
-        unfold expandBranch_one_component_sem_conform, ref2var ;
-        unfold expandBranch_one_component_sem_conform, ref2var in H2.
-        rewrite CELemmas.find_add_neq.
-        + simpl expandBranch_one_var_sem.
-          apply negbTE in i ; rewrite i.
-          replace (CE.find (nat_to_var (id * 3 + 1)) empty_cmap) with (@None def_expr) in H2 by (done).
-          exact H2.
-        + unfold CE.SE.eq.
-          move /eqP : i => i ; contradict i ; move /eqP : i => i.
-          rewrite -i in Hh1.
-          destruct h1.
-          - unfold ref2var in Hh1.
-            injection Hh1 ; clear Hh1 ; unfold nat_to_var ; intro Hh1.
-            assert (s0 * 3 + 1 == id * 3 + 1) by (rewrite -(bin_of_natK (s0 * 3 + 1)) Hh1 bin_of_natK eq_refl //).
-            rewrite addn1 addn1 eqSS eqn_pmul2r // in H3.
+      - assert (exists t : fgtyp, ft = Gtyp t) by admit.
+        destruct H1.
+        rewrite H1 ; rewrite H1 in IHss'.
+        exact IHss'.
+      - (* register is similar to variable *)
+        admit.
+      - (* memory is similar to variable *)
+        admit.
+    + (* Swire *)
+      assert (exists t : fgtyp, f = Gtyp t) by admit.
+      destruct H1.
+      rewrite H1.
+      destruct (CE.find (nat_to_var (s * 3 + 1)) ce_declarations) eqn: Halready_declared ; try done.
+      simpl expandBranch_fun.
+      destruct (expandBranch_fun ss ce_other_modules cm_previous) ; try done.
+      destruct p as [_ cm_result].
+      intro.
+      specialize IHss' with (id := id).
+      unfold ref2var ; unfold ref2var in IHss'.
+      destruct (eqVneq s id).
+      - rewrite e.
+        rewrite CELemmas.find_add_eq ; try rewrite /CE.SE.eq eq_refl //.
+        unfold aggr_typ, expandBranch_one_component_sem_conform, ref2var.
+        rewrite CELemmas.find_add_eq ; try rewrite /CE.SE.eq eq_refl //.
+        simpl expandBranch_one_var_sem.
+        rewrite eq_refl /expr_tree_to_def_expr eq_refl //.
+      - assert (~ CE.SE.eq (nat_to_var (id * 3 + 1)) (nat_to_var (s * 3 + 1))).
+              unfold CE.SE.eq.
+              contradict i.
+              move /eqP : i => i.
+              apply can_inj with (g := nat_of_bin) in i ;
+                    try apply bin_of_natK.
+              move /eqP : i => i.
+              rewrite eqn_add2r eqn_mul2r orFb in i.
+              move /eqP : i => i.
+              apply can_inj with (g := bin_of_nat) in i ;
+                    try apply nat_of_binK.
+              rewrite i eq_refl //.
+        rewrite CELemmas.find_add_neq ; try exact H2.
+        destruct (CE.find (nat_to_var (id * 3 + 1)) ce_declarations) ; try done.
+        destruct p as [comp_typ fcomp].
+        destruct comp_typ as [ft|reg|mem|] ; try done.
+        * assert (exists t : fgtyp, ft = Gtyp t) by admit.
+          destruct H3.
+          rewrite H3 ; rewrite H3 in IHss'.
+          destruct (orient_of_comp fcomp == Source) ; try done.
+          unfold expandBranch_one_component_sem_conform, ref2var ;
+          unfold expandBranch_one_component_sem_conform, ref2var in IHss'.
+          simpl expandBranch_one_var_sem.
+          rewrite CELemmas.find_add_neq ; try exact H2.
+          apply negbTE in i.
+          rewrite (eq_sym id) i.
+          exact IHss'.
+        * (* register is similar to variable *)
+          admit.
+        * (* memory is similar to variable *)
+          admit.
+    + (* Sreg *)
+      (* Sreg is similar to Swire *)
+      admit.
+    + (* Smem *)
+      (* Smem is similar to Swire *)
+      admit.
+    + (* Sinst s s0, i.e. s = identifier and s0 = type of the module. *)
+      rename s0 into mdl.
+      simpl expandBranch_fun.
+      destruct (expandBranch_fun ss ce_other_modules cm_previous) eqn: Hebf ;
+            try (destruct (CE.find mdl ce_other_modules) ;
+                 try done ;
+                 destruct p, c, f, (CE.find (nat_to_var (s * 3 + 1)) ce_declarations) ;
+                 done).
+      destruct p as [ss_result cm_result].
+      destruct (CE.find mdl ce_other_modules) eqn: Hmdl ; try done.
+      destruct p as [ss_result_mdl cm_result_mdl].
+      destruct ss_result_mdl ; try done.
+      destruct cm_result_mdl ; try done.
+      destruct (CE.find (nat_to_var (s * 3 + 1)) ce_declarations) eqn: Hs ; try done.
+      destruct (init_instance s mdl ce_other_modules cm_result) eqn: Hinit_instance ; try done.
+      intro.
+      specialize IHss' with (id := id).
+      unfold ref2var ; unfold ref2var in IHss'.
+      destruct (eqVneq s id).
+      - (* id now does not have a ground type but is part of the instance.
+           That means, it has type (Btyp ...) where each field has a ground type. *)
+        rewrite !e CELemmas.find_add_eq ; try rewrite /CE.SE.eq eq_refl //.
+        rewrite e in Hinit_instance.
+        unfold aggr_typ.
+        (* Now we should argue as follows:
+           1. (to simplify) the type f is some (Btyp f0),
+              where f0 is a list of ground type entries.
+              (This should be based on H1 and Hs0.)
+           2. induction over f0. *)
+        unfold expandBranch_precondition_ce in H0.
+        specialize H0 with (id := mdl).
+        unfold init_instance in Hinit_instance.
+        destruct (CE.find mdl ce_other_modules) ; try done.
+        destruct p.
+        destruct c0, f0 ; try discriminate.
+        destruct f1 ; try done.
+        injection Hmdl ; intro Hf0 ; clear Hmdl.
+        rewrite -Hf0 ; clear Hf0 f.
+        simpl expandBranch_one_component_sem_conform_flipped.
+        move : H0 c Hinit_instance.
+        simpl init_ref.
+        induction f0 ; try done.
+        simpl expandBranch_precondition_ce_module_fields ; intros.
+        destruct f0 ; try done.
+        simpl expandBranch_one_component_sem_conform_flipped_fields ;
+        simpl expandBranch_one_component_sem_conform_flipped_fields in IHf0.
+        simpl init_ref_bundle in Hinit_instance.
+        destruct f.
+        + rewrite eq_refl /expr_tree_to_def_expr /var_to_nat bin_of_natK.
+          (* Actually I am not sure whether “Sink” is the correct
+             orientation in Hinit_instance. *)
+          (*rewrite /var_to_nat bin_of_natK in Hinit_instance.*)
+          destruct (init_ref_bundle (Eid id) f1 Sink
+                     cm_result) eqn: Hirb ; try done.
+          injection Hinit_instance ; clear Hinit_instance ; intro Hinit_instance.
+          (* I don't know how to continue here... *)
+          admit.
+        + apply IHf0 ; try done.
+          destruct (init_ref_bundle (Eid id) f1 Sink cm_result) ; try done.
+          (* Here it again looks like the orientation in Hinit_instance should be different. *)
+          admit.
+      - rewrite CELemmas.find_add_neq.
+        * (* This can be proven using IHss' and Hinit_instance.
+             Similar to the above, we use that s != id and therefore
+             the relevant parts of cm_result and c are equal. *)
+          admit.
+        * unfold CE.SE.eq.
+          contradict i.
+          move /eqP : i => i.
+          apply can_inj with (g := nat_of_bin) in i ;
+                try apply bin_of_natK.
+          move /eqP : i => i.
+          rewrite eqn_add2r eqn_mul2r orFb in i.
+          move /eqP : i => i.
+          apply can_inj with (g := bin_of_nat) in i ;
+                try apply nat_of_binK.
+          rewrite i eq_refl //.
+    + (* Snode s h0 *)
+      simpl expandBranch_fun.
+      destruct (expandBranch_fun ss ce_other_modules cm_previous) ; try done.
+      destruct p as [ss_result cm_result].
+      (* expandBranch_one_component_sem_conform ignores the Snode statement,
+         so it should be possible to prove this based on IHss'. *)
+      admit.
+    + (* Sfcnct h1 h2 *)
+      simpl expandBranch_fun.
+      destruct (ref2var h0) eqn: Hh0 ; try done.
+      destruct (CE.find s ce_declarations) eqn: Hfinds ; try done.
+      destruct p as [comp_typ_s fcomp_s].
+      destruct comp_typ_s ; try done.
+      destruct f ; try done.
+      destruct (expandBranch_fun ss ce_other_modules cm_previous) ;
+      destruct (orient_of_comp fcomp_s == Source) eqn: Horient ; try done.
+      destruct p as [ss_result cm_result].
+      intro.
+      specialize IHss' with (id := id).
+      destruct (eqVneq (Eid id) h0).
+      - rewrite e Hh0 ; rewrite e Hh0 in IHss'.
+        destruct (CE.find s ce_declarations) ; try done.
+        destruct p as [comp_typ fcomp].
+        injection Hfinds ; clear Hfinds ; intros.
+        rewrite H2 H1 Horient ; rewrite H2 H1 Horient in IHss'.
+        simpl expandBranch_one_component_sem_conform.
+        rewrite Hh0 CELemmas.find_add_eq ; try (unfold CE.SE.eq ; done).
+        rewrite eq_refl /expr_tree_to_def_expr eq_refl //.
+      - unfold ref2var ; unfold ref2var in IHss'.
+        destruct (CE.find (nat_to_var (id * 3 + 1)) ce_declarations) eqn: Hfind ; try done.
+        destruct p as [comp_typ fcomp].
+        destruct comp_typ as [ft|reg|mem|] ; try done.
+        * assert (exists t : fgtyp, ft = Gtyp t) by admit.
+          destruct H1 as [t].
+          rewrite H1 ; rewrite H1 in IHss'.
+          destruct (orient_of_comp fcomp == Source) ; try done.
+          unfold expandBranch_one_component_sem_conform, ref2var ;
+          unfold expandBranch_one_component_sem_conform, ref2var in IHss'.
+          rewrite CELemmas.find_add_neq.
+          + simpl expandBranch_one_var_sem.
+            apply negbTE in i ; rewrite i.
+            exact IHss'.
+          + unfold CE.SE.eq.
+            move /eqP : i => i ; contradict i ; move /eqP : i => i.
+            rewrite -i in Hh0.
+            destruct h0.
+            - unfold ref2var in Hh0.
+              injection Hh0 ; clear Hh0 ; unfold nat_to_var ; intro Hh1.
+              assert (s0 * 3 + 1 == id * 3 + 1) by (rewrite -(bin_of_natK (s0 * 3 + 1)) Hh1 bin_of_natK eq_refl //).
+              rewrite addn1 addn1 eqSS eqn_pmul2r // in H2.
+              move /eqP : H2 => H2.
+              rewrite -(nat_of_binK s0) H2 nat_of_binK ; reflexivity.
+            - contradict Hh0.
+              clear.
+              simpl ref2var.
+              destruct (ref2var h0) ; try done.
+              injection ; unfold nat_to_var ; intro Hh1.
+              enough (2 == 1) by done.
+              replace 1 with ((id * 3 + 1) %% 3) at 2 by (rewrite modnD // modnMl //).
+              replace 2 with ((pair (var_to_nat s) s0 * 3 + 2) %% 3) at 1 by (rewrite modnD // modnMl //).
+              rewrite -(bin_of_natK (pair (var_to_nat s) s0 * 3 + 2)) Hh1 bin_of_natK eq_refl //.
+            - contradict Hh0.
+              clear.
+              simpl ref2var.
+              destruct (ref2var h0) ; try done.
+              injection ; unfold nat_to_var ; intro Hh1.
+              enough (0 == 1) by done.
+              replace 1 with ((id * 3 + 1) %% 3) by (rewrite modnD // modnMl //).
+              replace 0 with ((pair (var_to_nat s) n * 3 + 3) %% 3) at 1 by (rewrite modnD // modnMl //).
+              rewrite -(bin_of_natK (pair (var_to_nat s) n * 3 + 3)) Hh1 bin_of_natK eq_refl //.
+            - contradict Hh0.
+              simpl ref2var.
+              discriminate.
+        * (* register is similar to variable *)
+          admit.
+        * (* memory is similar to variable *)
+          admit.
+    + (* Sinvalid h0. This is similar to Sfcnct, so we can skip this case. *)
+      admit.
+    + rename h into stmt, h0 into cond, h1 into ss_true, h2 into ss_false.
+      (* Swhen cond ss_true ss_false *)
+      specialize expandBranch_correct_Swhen with (ce_other_modules := ce_other_modules) (s := Swhen cond ss_true ss_false).
+      unfold expandBranch_correct_hfstmt_seq, expandBranch_sem_conform in expandBranch_correct_Swhen.
+      destruct expandBranch_correct_Swhen as [IHss_true IHss_false].
+      specialize IHss_true with (ce_previous_declarations := ce_declarations).
+      specialize IHss_false with (ce_previous_declarations := ce_declarations).
+      destruct (expandBranch_precondition_declarations ss_true ce_other_modules
+        ce_declarations) as [ce_true_result|] eqn: Htrue_declarations ; try done.
+      destruct (expandBranch_precondition_declarations ss_false ce_other_modules
+        ce_declarations) as [ce_false_result|] eqn: Hfalse_declarations ; try done.
+      destruct (ce_has_no_double_declarations ce_declarations ce_true_result ce_false_result) eqn: Hno_double_declarations ; try done.
+      unfold combine_branches_ce.
+      simpl expandBranch_fun.
+      destruct (expandBranch_fun ss ce_other_modules cm_previous) eqn: Hebf_before ; try done.
+      destruct p as [ss_result cm_result].
+      specialize IHss_true with (cm_previous := cm_result).
+      specialize IHss_false with (cm_previous := cm_result).
+      destruct (expandBranch_fun ss_true ce_other_modules cm_result) eqn: Htrue_branch ; try done.
+      destruct p as [ss_true_result cm_true_result].
+      destruct (expandBranch_fun ss_false ce_other_modules cm_result) eqn: Hfalse_branch ; try done.
+      destruct p as [ss_false_result cm_false_result].
+      unfold combine_branches.
+      simpl snd.
+      intro.
+      specialize IHss' with (id := id).
+      assert (expandBranch_fun_declarations_correspondence ce_declarations cm_result)
+            by (apply (expandBranch_fun_declarations_preserve_correspondence ss ce_previous_declarations cm_previous)
+                with (ce_other_modules := ce_other_modules) (ss_result := ss_result) ; done).
+      assert (IHss_true' : match ref2var (Eid id) with
+                           | OK var =>
+                               match CE.find var ce_true_result with
+                               | Some (@Aggr_typ _ t, fcomp) =>
+                                   if orient_of_comp fcomp == Source
+                                   then expandBranch_one_component_sem_conform_flipped
+                                     (Eid id) t ss_true cm_true_result cm_result
+                                   else expandBranch_one_component_sem_conform
+                                     (Eid id) t ss_true cm_true_result cm_result
+                               | Some (Reg_typ reg, _) =>
+                                   expandBranch_one_component_sem_conform
+                                     (Eid id) (type reg) ss_true cm_true_result cm_result
+                               | Some (Mem_typ mem, _) =>
+                                   match type_of_mem mem with
+                                   | OK tom =>
+                                       expandBranch_one_component_sem_conform_flipped
+                                         (Eid id) tom ss_true cm_true_result cm_result
+                                   | Err _ => false
+                                   end
+                               | _ => true
+                               end
+                           | Err _ => true
+                           end)
+            by (apply IHss_true ; done).
+      clear IHss_true.
+      assert (IHss_false' : match ref2var (Eid id) with
+                            | OK var =>
+                                match CE.find var ce_false_result with
+                                | Some (@Aggr_typ _ t, fcomp) =>
+                                    if orient_of_comp fcomp == Source
+                                    then expandBranch_one_component_sem_conform_flipped
+                                      (Eid id) t ss_false cm_false_result cm_result
+                                    else expandBranch_one_component_sem_conform
+                                      (Eid id) t ss_false cm_false_result cm_result
+                                | Some (Reg_typ reg, _) =>
+                                    expandBranch_one_component_sem_conform
+                                      (Eid id) (type reg) ss_false cm_false_result cm_result
+                                | Some (Mem_typ mem, _) =>
+                                    match type_of_mem mem with
+                                    | OK tom =>
+                                        expandBranch_one_component_sem_conform_flipped
+                                          (Eid id) tom ss_false cm_false_result cm_result
+                                    | Err _ => false
+                                    end
+                                | _ => true
+                                end
+                            | Err _ => true
+                            end)
+            by (apply IHss_false ; done).
+      clear IHss_false.
+      unfold ref2var ; unfold ref2var in IHss' ;
+      unfold ref2var in IHss_true' ; unfold ref2var in IHss_false'.
+      (* In the following cases, we actually need something like:
+             ce_declarations contains an entry for (nat_to_var (id * 3 + 1))
+         iff cm_result       contains an entry for (nat_to_var (id * 3 + 1)). *)
+      assert (expandBranch_fun_declarations_correspondence ce_true_result cm_true_result)
+            by (apply (expandBranch_fun_declarations_preserve_correspondence ss_true ce_declarations cm_result)
+                with (ce_other_modules := ce_other_modules) (ss_result := ss_true_result) ; done).
+      assert (expandBranch_fun_declarations_correspondence ce_false_result cm_false_result)
+            by (apply (expandBranch_fun_declarations_preserve_correspondence ss_false ce_declarations cm_result)
+                with (ce_other_modules := ce_other_modules) (ss_result := ss_false_result) ; done).
+      unfold expandBranch_fun_declarations_correspondence in H1.
+      specialize H1 with (var := nat_to_var (id * 3 + 1)).
+      unfold expandBranch_fun_declarations_correspondence in H2.
+      specialize H2 with (var := nat_to_var (id * 3 + 1)).
+      unfold expandBranch_fun_declarations_correspondence in H3.
+      specialize H3 with (var := nat_to_var (id * 3 + 1)).
+      destruct (CE.find (nat_to_var (id * 3 + 1)) ce_declarations) eqn: Hfind_ce_before.
+      - (* id was declared before the Swhen statement. *)
+        assert (Hfind_ce_true : CE.find (nat_to_var (id * 3 + 1)) ce_true_result = Some p).
+              apply expandBranch_precondition_declarations_does_not_redefine
+                    with (ce_other_modules := ce_other_modules) (ss := ss_true)
+                         (ce_previous := ce_declarations) ; done.
+        rewrite Hfind_ce_true in IHss_true'.
+        rewrite Hfind_ce_true in H2.
+        assert (Hfind_ce_false : CE.find (nat_to_var (id * 3 + 1)) ce_false_result = Some p).
+              apply expandBranch_precondition_declarations_does_not_redefine
+                    with (ce_other_modules := ce_other_modules) (ss := ss_false)
+                         (ce_previous := ce_declarations) ; done.
+        rewrite Hfind_ce_false in IHss_false'.
+        rewrite Hfind_ce_false in H3.
+        rewrite CE.map2_1 ;
+              try (left ; exists p ; apply CE.find_2 ; exact Hfind_ce_true).
+        unfold combine_branches_ce_map2_helper.
+        rewrite Hfind_ce_true.
+        destruct p as [comp_typ fcomp].
+        destruct (orient_of_comp fcomp == Source) eqn: Horient.
+        * (* the orientation is Source, so it is in none of the cmaps. *)
+          destruct comp_typ as [ft|reg|mem|] ; try done.
+          + assert (exists t : fgtyp, ft = Gtyp t) by admit.
+            destruct H4 as [t] ; rewrite H4.
+            done.
+          + (* register is similar to variable *)
+            admit.
+          + (* memory is similar to variable *)
+            admit.
+        * (* the orientation is <> Source *)
+          destruct comp_typ as [ft|reg|mem|] ; try done.
+          + assert (exists t : fgtyp, ft = Gtyp t) by admit.
+            destruct H4 as [t] ; rewrite H4 ; rewrite H4 in IHss' ;
+            rewrite H4 in IHss_true' ; rewrite H4 in IHss_false'.
+            unfold expandBranch_one_component_sem_conform, ref2var ;
+            unfold expandBranch_one_component_sem_conform, ref2var in IHss' ;
+            unfold expandBranch_one_component_sem_conform, ref2var in IHss_true' ;
+            unfold expandBranch_one_component_sem_conform, ref2var in IHss_false'.
+            assert (exists d : def_expr, CE.find (nat_to_var (id * 3 + 1)) cm_result = Some d).
+                  destruct (CE.find (nat_to_var (id * 3 + 1)) cm_result) eqn: Hfind_cm_before.
+                  - exists d ; reflexivity.
+                  - rewrite eq_refl in H1 ; assert false by (apply H1 ; done) ; done.
+            destruct H5 as [de_before].
+            assert (exists d : def_expr, CE.find (nat_to_var (id * 3 + 1)) cm_true_result = Some d).
+                  destruct (CE.find (nat_to_var (id * 3 + 1)) cm_true_result) eqn: Hfind_cm_true.
+                  - exists d ; reflexivity.
+                  - rewrite eq_refl in H2 ; assert false by (apply H2 ; done) ; done.
+            destruct H6 as [de_true].
+            assert (exists d : def_expr, CE.find (nat_to_var (id * 3 + 1)) cm_false_result = Some d).
+                  destruct (CE.find (nat_to_var (id * 3 + 1)) cm_false_result) eqn: Hfind_cm_false.
+                  - exists d ; reflexivity.
+                  - rewrite eq_refl in H3 ; assert false by (apply H3 ; done) ; done.
+            destruct H7 as [de_false].
+            clear H1 H2 H3.
+            rewrite CE.map2_1.
+            - rewrite H6 H7.
+              unfold map2_helper_cs_tf.
+              simpl expandBranch_one_var_sem.
+              (* Here we need to run an induction over the structure of the expr_tree
+                 on the right-hand side of the equation.
+                 (“destruct” is not sufficient because T_choice contains trees again.)
+                 It should all be possible but it is long to write out the many cases... *)
+              admit.
+            - left.
+              destruct (CE.find (nat_to_var (id * 3 + 1)) cm_true_result) eqn: Hfind_cm_true ; try done.
+              exists d.
+              apply CE.find_2 ; exact Hfind_cm_true.
+          + (* register is similar to variable *)
+            admit.
+          + (* memory is similar to variable *)
+            admit.
+      destruct (CE.find (nat_to_var (id * 3 + 1)) ce_true_result) eqn: Hfind_ce_true.
+      - (* id was declared in the true branch.
+           We know that it was not declared in the false branch. *)
+        rewrite CE.map2_1 ;
+              try (left ;
+                   unfold CE.In ;
+                   exists p ;
+                   apply CE.find_2, Hfind_ce_true).
+        rewrite /combine_branches_ce_map2_helper Hfind_ce_true.
+        destruct p as [comp_typ_true fcomp_true].
+        assert (Hfind_ce_false : CE.find (nat_to_var (id * 3 + 1)) ce_false_result = None).
+              (* should follow from type correctness of declarations:
+                 a component cannot be declared in both branches of a Swhen statement *)
+              apply CE.is_empty_2 in Hno_double_declarations.
+              unfold CE.Empty in Hno_double_declarations.
+              destruct (CE.find (nat_to_var (id * 3 + 1)) ce_false_result) eqn: Hfind_ce_false ; try done.
+              destruct p as [comp_typ_false fcomp_false].
+              specialize Hno_double_declarations with (a := (nat_to_var (id * 3 + 1))) (e := (comp_typ_true, fcomp_true)).
+              contradict Hno_double_declarations.
+              apply CE.find_2.
+              rewrite CE.map2_1.
+              + rewrite CE.map2_1 ;
+                      try (left ; exists (comp_typ_true, fcomp_true) ;
+                           apply CE.find_2, Hfind_ce_true).
+                rewrite CE.map2_1 ;
+                      try (left ; exists (comp_typ_false, fcomp_false) ;
+                           apply CE.find_2, Hfind_ce_false).
+                rewrite Hfind_ce_true Hfind_ce_false Hfind_ce_before
+                        /ce_map_difference_helper
+                        /ce_map_intersection_helper //.
+              + left.
+                exists (comp_typ_true, fcomp_true).
+                apply CE.find_2.
+                rewrite CE.map2_1 ;
+                      try (left ; exists (comp_typ_true, fcomp_true) ;
+                           apply CE.find_2, Hfind_ce_true).
+                rewrite /ce_map_difference_helper Hfind_ce_before Hfind_ce_true //.
+        rewrite Hfind_ce_false in H3.
+        destruct (orient_of_comp fcomp_true == Source) eqn: Horient.
+        * (* the orientation is Source, so it is in none of the cmaps. *)
+          destruct comp_typ_true as [ft|reg|mem|] ; try done.
+          + assert (exists t : fgtyp, ft = Gtyp t) by admit.
+            destruct H4 as [t] ; rewrite H4.
+            done.
+          + (* register is similar to variable *)
+            admit.
+          + (* memory is similar to variable *)
+            admit.
+        * (* the orientation is <> Source *)
+          destruct comp_typ_true as [ft|reg|mem|] ; try done.
+          + assert (exists t : fgtyp, ft = Gtyp t) by admit.
+            destruct H4 as [t] ; rewrite H4 ; rewrite H4 in IHss_true'.
+            unfold expandBranch_one_component_sem_conform, ref2var ;
+            unfold expandBranch_one_component_sem_conform, ref2var in IHss_true'.
+            move /eqP : H1 => H1.
+            assert (CE.find (nat_to_var (id * 3 + 1)) cm_previous = None) by admit.
+                  (* This should be proven based on the preservation of correspondence and H1. *)
+            assert (exists d : def_expr, CE.find (nat_to_var (id * 3 + 1)) cm_true_result = Some d).
+                  destruct (CE.find (nat_to_var (id * 3 + 1)) cm_true_result) eqn: Hfind_cm_true.
+                  - exists d ; reflexivity.
+                  - rewrite eq_refl in H2 ; assert false by (apply H2 ; done) ; done.
+            destruct H6 as [de_true].
+            clear H2.
             move /eqP : H3 => H3.
-            rewrite -(nat_of_binK s0) H3 nat_of_binK ; reflexivity.
-          - contradict Hh1.
-            clear.
-            simpl ref2var.
-            destruct (ref2var h1) ; try done.
-            injection ; unfold nat_to_var ; intro Hh1.
-            enough (2 == 1) by done.
-            replace 1 with ((id * 3 + 1) %% 3) at 2 by (rewrite modnD // modnMl //).
-            replace 2 with ((pair (var_to_nat s) s0 * 3 + 2) %% 3) at 1 by (rewrite modnD // modnMl //).
-            rewrite -(bin_of_natK (pair (var_to_nat s) s0 * 3 + 2)) Hh1 bin_of_natK eq_refl //.
-          - contradict Hh1.
-            clear.
-            simpl ref2var.
-            destruct (ref2var h1) ; try done.
-            injection ; unfold nat_to_var ; intro Hh1.
-            enough (0 == 1) by done.
-            replace 1 with ((id * 3 + 1) %% 3) by (rewrite modnD // modnMl //).
-            replace 0 with ((pair (var_to_nat s) n * 3 + 3) %% 3) at 1 by (rewrite modnD // modnMl //).
-            rewrite -(bin_of_natK (pair (var_to_nat s) n * 3 + 3)) Hh1 bin_of_natK eq_refl //.
-          - contradict Hh1.
-            simpl ref2var.
-            discriminate.
-      * (* register is similar to variable *)
+            rewrite CE.map2_1.
+            - rewrite H6 H3 H5.
+              rewrite H1 in IHss_true'.
+              unfold map2_helper_cs_tf.
+              simpl expandBranch_one_var_sem.
+              assert (expandBranch_one_var_sem ss (Eid id) T_undeclared = T_undeclared) by admit.
+                    (* This should hold because the variable was not declared before the true branch.
+                       I think that a slight change in IHss' should entail this. *)
+              assert (expandBranch_one_var_sem ss_false (Eid id) T_undeclared = T_undeclared) by admit.
+              rewrite H2 H7.
+              rewrite H6 in IHss_true'.
+              destruct de_true, (expandBranch_one_var_sem ss_true (Eid id) T_undeclared) ;
+                    exact IHss_true'.
+            - left.
+              destruct (CE.find (nat_to_var (id * 3 + 1)) cm_true_result) eqn: Hfind_cm_true ; try done.
+              exists d.
+              apply CE.find_2 ; exact Hfind_cm_true.
+          + (* register is similar to variable *)
+            admit.
+          + (* memory is similar to variable *)
+            admit.
+      destruct (CE.find (nat_to_var (id * 3 + 1)) ce_false_result) eqn: Hfind_ce_false.
+      - (* id was declared in the false branch.
+           Similar to the above (true branch). *)
         admit.
-      * (* memory is similar to variable *)
-        admit.
-  + (* Sinvalid h1. This is similar to Sfcnct, so we can skip this case. *)
-    admit.
-  + rename h into ss_butlast, h0 into stmt, h1 into cond, h2 into ss_true, h3 into ss_false.
-    (* Swhen cond ss_true ss_false, where h1 is a condition and h2 and h3 are statement sequences. *)
-    destruct (expandBranch_precondition_declarations ss_true ce_other_modules
-      ce_declarations) as [ce_true_result|] eqn: Htrue_declarations ; try done.
-    destruct (expandBranch_precondition_declarations ss_false ce_other_modules
-      ce_true_result) as [ce_false_result|] eqn: Hfalse_declarations ; try done.
-    simpl expandBranch_fun.
-    destruct (expandBranch_fun ss_butlast ce_other_modules empty_cmap) ; try done.
-    destruct p as [_ cm_result].
-    destruct (expandBranch_fun ss_true ce_other_modules cm_result) eqn: Htrue_branch ; try done.
-    destruct (expandBranch_fun ss_false ce_other_modules cm_result) eqn: Hfalse_branch ; try done.
-    unfold combine_branches.
-    destruct p as [ss_true_result cm_true_result].
-    destruct p0 as [ss_false_result cm_false_result].
-    simpl snd.
-    intro.
-    specialize H2 with (id := id).
-    unfold ref2var ; unfold ref2var in H2.
-    (* In the following cases, we actually need something like:
-           ce_declarations contains an entry for (nat_to_var (id * 3 + 1))
-       iff cm_result       contains an entry for (nat_to_var (id * 3 + 1)). *)
-(*
-ce_declarations contains declarations from both branches (true and false branch).
-cm_result is constructed first using only one branch,
-and then the two variants of cm_result are combined with combine_branches.
-
-ce_declarations is generated by a function that is part of the specification.
-cm_result is generated by expandBranch_fun (the actual translation function).
-*)
-    destruct (CE.find (nat_to_var (id * 3 + 1)) ce_declarations) eqn: Hfind_s_before.
-    - (* id was declared before the Swhen statement. *)
-      assert (Hfind_s_after : CE.find (nat_to_var (id * 3 + 1)) ce_false_result = Some p).
-            apply expandBranch_precondition_declarations_does_not_redefine
-                  with (ce_other_modules := ce_other_modules) (ss := ss_false)
-                       (ce_previous := ce_true_result) ; try done.
-            apply expandBranch_precondition_declarations_does_not_redefine
-                  with (ce_other_modules := ce_other_modules) (ss := ss_true)
-                       (ce_previous := ce_declarations) ; done.
-      rewrite Hfind_s_after.
-      destruct p as [comp_typ fcomp].
-      destruct comp_typ as [ft|reg|mem|] ; try done.
-      * assert (exists t : fgtyp, ft = Gtyp t) by admit.
-        destruct H as [t] ; rewrite H ; rewrite H in H2.
-        simpl expandBranch_one_component_sem_conform ;
-        simpl expandBranch_one_component_sem_conform in H2.
-        rewrite CE.map2_1.
-        - admit.
-        - (* Because of Hfind_s_before, we should be able to deduce
-             that cm_result also contains a definition.
-             Then, cm_true_result and cm_false_result also contain definitions. *)
-          admit.
-      * (* register is similar to variable *)
-        admit.
-      * (* memory is similar to variable *)
-        admit.
-    destruct (CE.find (nat_to_var (id * 3 + 1)) ce_true_result) eqn: Hfind_s_true.
-    - (* id was only declared in the true branch of the Swhen statement. *)
-      assert (Hfind_s_after : CE.find (nat_to_var (id * 3 + 1)) ce_false_result = Some p).
-            apply expandBranch_precondition_declarations_does_not_redefine
-                  with (ce_other_modules := ce_other_modules) (ss := ss_false)
-                       (ce_previous := ce_true_result) ; done.
-      rewrite Hfind_s_after.
-      destruct p as [comp_typ fcomp].
-      destruct comp_typ as [ft|reg|mem|] ; try done.
-      * assert (exists t : fgtyp, ft = Gtyp t) by admit.
-        destruct H as [t] ; rewrite H.
-        simpl expandBranch_one_component_sem_conform.
-        rewrite CE.map2_1.
-        - admit.
-        - (* Because of Hfind_s_true, we should be able to deduce
-             that cm_true_result also contains a definition. *)
-          left.
-          admit.
-      * (* register is similar to variable *)
-        admit.
-      * (* memory is similar to variable *)
-        admit.
-    destruct (CE.find (nat_to_var (id * 3 + 1)) ce_false_result) eqn: Hfind_s_false.
-    - (* id was only declared in the false branch of the Swhen statement. *)
-      destruct p as [comp_typ fcomp].
-      destruct comp_typ as [ft|reg|mem|] ; try done.
-      * assert (exists t : fgtyp, ft = Gtyp t) by admit.
-        destruct H as [t] ; rewrite H.
-        simpl expandBranch_one_component_sem_conform.
-        rewrite CE.map2_1.
-        - admit.
-        - (* Because of Hfind_s_false, we should be able to deduce
-             that cm_false_result also contains a definition. *)
-          right.
-          admit.
-      * (* register is similar to variable *)
-        admit.
-      * (* memory is similar to variable *)
-        admit.
-    - (* id was only declared after the Swhen statement. *)
-      done.
+      - assert (~CE.In (nat_to_var (id * 3 + 1)) (CE.map2 combine_branches_ce_map2_helper ce_true_result
+                                                  ce_false_result)).
+              contradict IHss'.
+              apply CE.map2_2 in IHss'.
+              destruct IHss' ;
+                    unfold CE.In in H4 ;
+                    destruct H4 ;
+                    apply CE.find_1 in H4.
+              * rewrite H4 in Hfind_ce_true ; discriminate.
+              * rewrite H4 in Hfind_ce_false ; discriminate.
+        destruct (CE.find (nat_to_var (id * 3 + 1))
+                      (CE.map2 combine_branches_ce_map2_helper ce_true_result
+                       ce_false_result)) eqn: Hfind ;
+              try rewrite Hfind //.
+        absurd (CE.In (nat_to_var (id * 3 + 1))
+              (CE.map2 combine_branches_ce_map2_helper ce_true_result
+                       ce_false_result)) ; try done.
+        apply CE.find_2 in Hfind.
+        exists p ; exact Hfind.
+* clear expandBranch_correct_Swhen.
+  destruct s ; done.
 Admitted.
 
 
